LeanSAT/Reflect/BVExpr/BitBlast/Impl/RotateRight.lean
@@ -1,0 +1,50 @@
+import LeanSAT.Reflect.BVExpr.Basic
+import LeanSAT.AIG
+
+namespace BVExpr
+namespace bitblast
+
+/-
+@[simp]
+theorem getLsb_rotateRight {x : BitVec w} {r i : Nat} :
+    (x.rotateRight r).getLsb i =
+      cond (i < w - (r % w))
+      (x.getLsb ((r % w) + i))
+      (decide (i < w) && x.getLsb (i - (w - (r % w))))
+-/
+
+def blastRotateRight (aig : AIG BVBit) (target : AIG.ShiftTarget aig w)
+    : AIG.RefStreamEntry BVBit w :=
+  let ⟨input, distance⟩ := target
+  ⟨aig, go input distance 0 (by omega) .empty⟩
+where
+  go {aig : AIG BVBit} (input : AIG.RefStream aig w) (distance : Nat) (curr : Nat) (hcurr : curr ≤ w)
+      (s : AIG.RefStream aig curr)
+    : AIG.RefStream aig w :=
+  if hcurr1:curr < w then
+    if hcurr2:curr < w - distance % w then
+      let ref := input.getRef ((distance % w) + curr) (by omega)
+      let s := s.pushRef ref
+      go input distance (curr + 1) (by omega) s
+    else
+      let ref := input.getRef (curr - (w - (distance % w))) (by omega)
+      let s := s.pushRef ref
+      go input distance (curr + 1) (by omega) s
+  else
+    have hcurr : curr = w := by omega
+    hcurr ▸ s
+termination_by w - curr
+
+instance : AIG.LawfulStreamOperator BVBit AIG.ShiftTarget blastRotateRight where
+  le_size := by
+    intros
+    unfold blastRotateRight
+    dsimp
+    omega
+  decl_eq := by
+    intros
+    unfold blastRotateRight
+    dsimp
+
+end bitblast
+end BVExpr
